Zmodule base theory

theories/Ring.ec
@@ -3,6 +3,97 @@
  * -------------------------------------------------------------------- *)
 
 (* -------------------------------------------------------------------- *)
+theory ZModule.
+  require import Fun.
+
+  type zmodule.
+
+  op zeror : zmodule.
+
+  op ( + ) : zmodule -> zmodule -> zmodule.
+  op [ - ] : zmodule -> zmodule.
+
+  op ( - ) (x y : zmodule) = x + -y axiomatized by subrE.
+
+  axiom nosmt addrA (x y z : zmodule): x + (y + z) = (x + y) + z.
+  axiom nosmt addrC (x y   : zmodule): x + y = y + x.
+  axiom nosmt add0r (x     : zmodule): zeror + x = x.
+  axiom nosmt addNr (x     : zmodule): (-x) + x = zeror.
+
+  lemma nosmt addr0 (x : zmodule): x + zeror = x.
+  proof. by rewrite addrC add0r. qed.
+
+  lemma nosmt addrN (x : zmodule): x + (-x) = zeror.
+  proof. by rewrite addrC addNr. qed.
+
+  lemma addrCA (x y z): x + (y + z) = y + (x + z).
+  proof. by rewrite !addrA (addrC x y). qed.
+
+  lemma addrAC (x y z): (x + y) + z = (x + z) + y.
+  proof. by rewrite -!addrA (addrC y z). qed.
+
+  lemma nosmt subrr (x : zmodule): x - x = zeror.
+  proof. by rewrite subrE /= addrN. qed.
+
+  lemma nosmt addKr (x y : zmodule): -x + (x + y) = y.
+  proof. by rewrite addrA addNr add0r. qed.
+
+  lemma nosmt addNKr (x y : zmodule): x + (-x + y) = y.
+  proof. by rewrite addrA addrN add0r. qed.
+
+  lemma nosmt addrK (y x : zmodule): (x + y) + -y = x.
+  proof. by rewrite -addrA addrN addr0. qed.
+
+  lemma nosmt addrNK (x y : zmodule): (x + -y) + y = x.
+  proof. by rewrite -addrA addNr addr0. qed.
+
+  lemma nosmt addrI (x y z : zmodule): x + y = x + z => y = z.
+  proof. cut := addKr x; smt. qed.
+
+  lemma nosmt addIr (x y z : zmodule): y + x = z + x => y = z.
+  proof. cut := addrK x; smt. qed.
+
+  lemma nosmt opprK (x : zmodule): -(-x) = x.
+  proof. by apply (addIr (-x)); rewrite addNr addrN. qed.
+
+  lemma nosmt oppr0: -zeror = zeror.
+  proof. by rewrite -(addr0 (-zeror)) addNr. qed.
+
+  lemma nosmt subr0 (x : zmodule): x - zeror = x.
+  proof. by rewrite subrE /= oppr0 addr0. qed.
+
+  lemma nosmt sub0r (x : zmodule): zeror - x = - x.
+  proof. by rewrite subrE /= add0r. qed.
+
+  lemma nosmt opprD (x y : zmodule): -(x + y) = -x + -y.
+  proof.
+    by apply (addrI (x + y)); rewrite addrA addrN addrAC addrK addrN.
+  qed.
+
+  lemma nosmt opprB (x y : zmodule): -(x - y) = y - x.
+  proof. by rewrite subrE /= opprD opprK addrC. qed.
+
+  lemma nosmt subr_eq x y z : (x - z = y) <=> (x = y + z).
+  proof.
+    move: (can2_eq (fun x, x - z) (fun x, x + z) _ _ x y) => //=.
+    by move=> {x} x /=; rewrite subrE /= addrNK.
+    by move=> {x} x /=; rewrite subrE /= addrK.
+  qed.
+
+  lemma nosmt subr_eq0 (x y : zmodule): (x - y = zeror) <=> (x = y).
+  proof. by rewrite subr_eq add0r. qed.
+
+  lemma nosmt addr_eq0 (x y : zmodule): (x + y = zeror) <=> (x = -y).
+  proof. by rewrite -(subr_eq0 x) subrE /= opprK. qed.
+
+  lemma nosmt eqr_opp (x y : zmodule): (- x = - y) <=> (x = y).
+  proof.
+    move: (can_eq (fun z, -z) (fun z, -z) _ x y) => //=.
+    by move=> z /=; rewrite opprK.
+  qed.
+end ZModule.
+
+(* -------------------------------------------------------------------- *)
 theory R.
   require import Fun.
 
